

## 性质1

$$
\tag{1.38}\forall{i},P(v_i\mid pa_i)=P_{pa_i}(v_i)
$$

证明：
$$
\because V_i\cancel{\in}PA_i,根据定义（1.3.1）条件(iii)得到：
\tag{1}P(v_i\mid pa_i)=P_{pa_i}(v_i\mid pa_i)=\frac{P_{pa_i}(v_i,pa_i)}{P_{pa_i}(pa_i)}
$$

$$
条件（ii），\tag{2}P_{pa_i}(pa_i)\equiv1
$$

$$
\tag{3}P_{pa_i}(v_i,pa_1)\equiv{P_{pa_i}}(v_i)
$$

结合1，2，3可得结论。



##性质2
$$
\forall{i},\forall{S\subset{V}}，满足S\land(V_i,PA_i)=\empty,以下成立
$$

$$
P_{pa_i,s}(v_i)=P_{pa_i}(v_i)
$$

证明：
$$
由条件（ii）P_{pa_i,s}(pa_i)=1，故P_{pa_i,s}(v_1)=P_{pa_i,s}(v_i,pa_i)
$$

$$
可得：P_{pa_i,s}(v_1)=\frac{P_{pa_i,s}(v_i,pa_i)}{P_{pa_i,s}(pa_i)}=P_{pa_i,s}(v_1\mid{pa_i})
$$

$$
V_i\cancel\in(PA_i,S),根据条件(iii),P_{pa_i,s}(v_1\mid{pa_i})=P(v_1\mid{pa_i})
$$

结合刚刚证的性质1，结论可得。