

## 性质1

$$
\tag{1.38}\mathit{\forall{i},P(v_i\mid pa_i)=P_{pa_i}(v_i)}
$$

证明：
$$
\because \mathit{V_i \notin PA_i},根据定义（1.3.1）条件(iii)得到：
\tag{1}\mathit{P(v_i\mid pa_i)=P_{pa_i}(v_i\mid pa_i)=\frac{P_{pa_i}(v_i,pa_i)}{P_{pa_i}(pa_i)}}
$$

$$
条件（ii），\tag{2}\mathit{P_{pa_i}(pa_i)\equiv1}
$$

$$
\tag{3}\mathit{P_{pa_i}(v_i,pa_1)\equiv{P_{pa_i}}(v_i)}
$$

结合1，2，3可得结论。 $\blacksquare$





## 性质2


$$
\mathit{\forall{i},\forall{S\subset{V}}}，满足\mathit{S\land\{V_i,PA_i\}=\empty},以下成立
$$

$$
\mathit{P_{pa_i,s}(v_i)=P_{pa_i}(v_i）}
$$

证明：
$$
由条件（ii）\mathit{P_{pa_i,s}(pa_i)=1}，故\mathit{P_{pa_i,s}(v_1)=P_{pa_i,s}(v_i,pa_i)}
$$

$$
可得：\mathit{P_{pa_i,s}(v_1)=\frac{P_{pa_i,s}(v_i,pa_i)}{P_{pa_i,s}(pa_i)}=P_{pa_i,s}(v_1\mid{pa_i})}
$$

$$
\mathit{V_i \notin \{PA_i,S\}},根据条件(iii)，\mathit{P_{pa_i,s}(v_1\mid{pa_i})=P(v_1\mid{pa_i})}
$$

结合刚刚证的性质1，可得结论。$\blacksquare$

